feat: seqMap

Arithmetization/ISigmaOne/HFS.lean
@@ -1,4 +1,5 @@
 import Arithmetization.ISigmaOne.Bit
+import Arithmetization.Vorspiel.ExistsUnique
 
 /-!
 
@@ -525,6 +526,14 @@ lemma mem_seqCons_iff {i x z s : M} : ⟪i, x⟫ ∈ z ::ˢ s ↔ (i = lh s ∧ 
 
 @[simp] lemma lh_mem_seqCons (s z : M) : ⟪lh s, z⟫ ∈ z ::ˢ s := by simp [seqCons]
 
+@[simp] lemma lh_mem_seqCons_iff {s x z : M} (H : Seq s) : ⟪lh s, x⟫ ∈ z ::ˢ s ↔ x = z := by
+  simp [seqCons]
+  intro h; have := H.lt_lh_of_mem h; simp at this
+
+lemma Seq.mem_seqCons_iff_of_lt {s x z : M} (H : Seq s) (hi : i < lh s) : ⟪i, x⟫ ∈ z ::ˢ s ↔ ⟪i, x⟫ ∈ s := by
+  simp [seqCons, hi]
+  rintro rfl; simp at hi
+
 lemma domain_bitRemove_of_isMapping_of_mem {x y s : M} (hs : IsMapping s) (hxy : ⟪x, y⟫ ∈ s) :
     domain (bitRemove ⟪x, y⟫ s) = bitRemove x (domain s) := by
   apply mem_ext; simp [mem_domain_iff]; intro x₁
@@ -532,6 +541,19 @@ lemma domain_bitRemove_of_isMapping_of_mem {x y s : M} (hs : IsMapping s) (hxy :
   · rintro ⟨y₁, hy₁, hx₁y₁⟩; exact ⟨by rintro rfl; exact hy₁ rfl (hs.uniq hx₁y₁ hxy), y₁, hx₁y₁⟩
   · intro ⟨hx, y₁, hx₁y₁⟩
     exact ⟨y₁, by intro _; contradiction, hx₁y₁⟩
+
+lemma Seq.eq_of_eq_of_subset {s₁ s₂ : M} (H₁ : Seq s₁) (H₂ : Seq s₂)
+    (hl : lh s₁ = lh s₂) (h : s₁ ⊆ s₂) : s₁ = s₂ := by
+  apply mem_ext; intro u
+  constructor
+  · intro hu; exact h hu
+  · intro hu
+    have : π₁ u < lh s₁ := by simpa [hl] using H₂.lt_lh_of_mem (show ⟪π₁ u, π₂ u⟫ ∈ s₂ from by simpa using hu)
+    have : ∃ y, ⟪π₁ u, y⟫ ∈ s₁ := H₁.exists this
+    rcases this with ⟨y, hy⟩
+    have : y = π₂ u := H₂.isMapping.uniq (h hy) (show ⟪π₁ u, π₂ u⟫ ∈ s₂ from by simpa using hu)
+    rcases this with rfl
+    simpa using hy
 
 /-- TODO: move to Lemmata.lean-/
 lemma ne_zero_iff_one_le {a : M} : a ≠ 0 ↔ 1 ≤ a := Iff.trans pos_iff_ne_zero.symm (pos_iff_one_le (a := a))
@@ -568,7 +590,8 @@ alias ⟨Seq.cases, _⟩ := Seq.cases_iff
     {P : M → Prop} (hP : DefinablePred ℒₒᵣ (Γ, 1) P)
     (ind : ∀ x, (∀ y < x, P y) → P x) : ∀ x, P x := order_induction_hh ℒₒᵣ Γ 1 hP ind
 
-theorem seq_induction {P : M → Prop} (hP : DefinablePred ℒₒᵣ (Γ, 1) P)
+@[elab_as_elim]
+theorem seq_induction (Γ) {P : M → Prop} (hP : DefinablePred ℒₒᵣ (Γ, 1) P)
   (hnil : P ∅) (hcons : ∀ s x, Seq s → P s → P (x ::ˢ s)) :
     ∀ {s : M}, Seq s → P s := by
   intro s sseq
@@ -597,6 +620,111 @@ def vecConsUnexpander : Lean.PrettyPrinter.Unexpander
   | _ => throw ()
 
 @[simp] lemma singleton_seq (x : M) : Seq !⟨x⟩ := by apply Seq.seqCons; simp
+
+section seqMap
+
+variable {f : M → M} (hf : 𝚺₁-Function₁ f)
+
+lemma Seq.seqMap_exists {s : M} (Hs : Seq s) :
+    ∃ t, Seq t ∧ lh t = lh s ∧ ∀ i x, ⟪i, x⟫ ∈ s → ⟪i, f x⟫ ∈ t := by
+  suffices ∃ t, Seq t ∧ lh t = lh s ∧ ∀ i < lh s, ∀ x < s, ⟪i, x⟫ ∈ s → ⟪i, f x⟫ ∈ t
+  by  rcases this with ⟨t, Ht, hts, h⟩
+      exact ⟨t, Ht, hts, fun i x hx ↦ h i (Hs.lt_lh_of_mem hx) x (lt_of_mem_rng hx) hx⟩
+  revert Hs
+  apply @seq_induction M _ _ _ _ _ _ 𝚺
+  · definability
+  case hnil =>
+    exact ⟨∅, by simp⟩
+  case hcons =>
+    intro s x Hs ⟨t, Ht, hts, ih⟩
+    exact ⟨f x ::ˢ t, Ht.seqCons (f x), by simp [Hs, Ht, hts], by
+      simp [Hs, Ht]
+      intro i hi z _ hz
+      have : i ≤ lh s := lt_succ_iff_le.mp hi
+      rcases this with (rfl | hi)
+      · have : z = x := by simpa [Hs] using hz
+        simp [this, ←hts, Ht]
+      · simp [Ht.mem_seqCons_iff_of_lt (by simpa [hts] using hi), Hs.mem_seqCons_iff_of_lt hi] at hz ⊢
+        exact ih i hi z (lt_of_mem_rng hz) hz ⟩
+
+lemma seqMap_existsUnique (s : M) (Hs : Seq s) :
+    ∃! t, Seq t ∧ lh t = lh s ∧ ∀ i x, ⟪i, x⟫ ∈ s → ⟪i, f x⟫ ∈ t := by
+  rcases Hs.seqMap_exists hf with ⟨t, Ht, hts, h⟩
+  apply ExistsUnique.intro t ⟨Ht, hts, h⟩
+  rintro t' ⟨Ht', ht's, h'⟩
+  apply Ht'.eq_of_eq_of_subset Ht (by simp [hts, ht's])
+  intro u hu
+  have : π₁ u < lh s := by simpa [←ht's] using Ht'.lt_lh_of_mem (show ⟪π₁ u, π₂ u⟫ ∈ t' from by simpa using hu)
+  have : ∃ y, ⟪π₁ u, y⟫ ∈ s := Hs.exists this
+  rcases this with ⟨y, hy⟩
+  have : f y = π₂ u := Ht'.isMapping.uniq (h' _ _ hy) (show ⟪π₁ u, π₂ u⟫ ∈ t' from by simpa using hu)
+  simpa [this] using h _ _ hy
+
+def seqMap (s : M) : M := Classical.extendedChoose! (seqMap_existsUnique hf) 0 s
+
+lemma Seq.seqMap_spec' {s : M} (H : Seq s) :
+    Seq (seqMap hf s) ∧ lh (seqMap hf s) = lh s ∧ ∀ i x, ⟪i, x⟫ ∈ s → ⟪i, f x⟫ ∈ seqMap hf s :=
+  Classical.extendedchoose!_spec (seqMap_existsUnique hf) 0 H
+
+@[simp] lemma seqMap_spec_of_not_seq {s : M} (H : ¬Seq s) :
+    seqMap hf s = 0 :=
+  Classical.extendedchoose!_spec_not (seqMap_existsUnique hf) 0 H
+
+variable {hf} {s : M} (H : Seq s)
+
+@[simp] protected lemma Seq.seqMap : Seq (seqMap hf s) := H.seqMap_spec' hf |>.1
+
+@[simp] lemma Seq.seqMap_lh_eq : lh (seqMap hf s) = lh s := H.seqMap_spec' hf |>.2.1
+
+lemma Seq.seqMap_spec {i x : M} : ⟪i, x⟫ ∈ s → ⟪i, f x⟫ ∈ seqMap hf s := H.seqMap_spec' hf |>.2.2 i x
+
+lemma Seq.mem_seqMap_iff {i y : M} : ⟪i, y⟫ ∈ seqMap hf s ↔ ∃ x, f x = y ∧ ⟪i, x⟫ ∈ s :=
+  ⟨by intro hu
+      have : i < lh s := by simpa [H] using H.seqMap.lt_lh_of_mem hu
+      have : ∃ x, ⟪i, x⟫ ∈ s := H.exists this
+      rcases this with ⟨x, hx⟩
+      exact ⟨x, H.seqMap.isMapping.uniq (H.seqMap_spec hx) hu, hx⟩,
+   by rintro ⟨x, rfl, hx⟩; exact H.seqMap_spec hx⟩
+
+lemma seqMap_graph (t s : M) :
+    t = seqMap hf s ↔
+    (Seq s → Seq t ∧ (∃ l < 2 * s + 1, l = lh s ∧ l = lh t) ∧ ∀ i < s, ∀ x < s, ⟪i, x⟫ ∈ s → ∃ y < t, y = f x ∧ ⟪i, y⟫ ∈ t) ∧
+    (¬Seq s → t = 0) :=
+  ⟨by rintro rfl;
+      by_cases H : Seq s <;> simp only [H, Seq.seqMap, lt_succ_iff_le, Seq.seqMap_lh_eq, and_self,
+        exists_eq_right, lh_bound, true_and, forall_true_left, not_true_eq_false, IsEmpty.forall_iff, and_true,
+        not_false_eq_true, H, seqMap_spec_of_not_seq, forall_true_left]
+      intro i _ x _ hix
+      have : ⟪i, f x⟫ ∈ seqMap hf s := H.seqMap_spec hix
+      exact ⟨f x, lt_of_mem_rng this, rfl, this⟩,
+   by by_cases H : Seq s <;>
+        simp only [H, lt_succ_iff_le, exists_eq_right_right, forall_true_left,
+          not_true_eq_false, IsEmpty.forall_iff, and_true, and_imp]
+      intro Ht _ hl h
+      apply Classical.extendedChoose!_uniq
+      · exact H
+      · exact ⟨Ht, hl, by intro i x hi; rcases h i (lt_of_mem_dom hi) x (lt_of_mem_rng hi) hi with ⟨_, _, rfl, h⟩; exact h⟩
+      · simp [H]⟩
+
+end seqMap
+
+section seqMap₀
+
+variable (p : HSemisentence ℒₒᵣ 2 𝚺₀)
+
+def _root_.LO.FirstOrder.Arith.seqMap₀Def : 𝚺₀-Semisentence 2 := .mkSigma
+  “ ( !seqDef.val [#1] →
+      !seqDef.val [#0] ∧
+      (  ∃[#0 < 2 * #2 + 1] (  !lhDef.val [#0, #2] ∧ !lhDef.val [#0, #1]  )  ) ∧
+      ∀[#0 < #2] ∀[#0 < #3] ( #1 ~[#3] #0 → ∃[#0 < #3] ( !p.val [#0, #1] ∧ #2 ~[#3] #0 ) ) ) ∧
+    ( ¬!seqDef.val [#1] → #0 = 0 )” (by simp)
+
+variable {p} {f : M → M} (hf : 𝚺₀-Function₁ f via p)
+
+lemma seqMap₀_defined : 𝚺₀-Function₁ (seqMap (f := f) (Definable.of_zero hf.to_definable _) : M → M) via (seqMap₀Def p) := by
+  intro v; simp [seqMap₀Def, seqMap_graph, hf.df.iff]
+
+end seqMap₀
 
 end seq
 
