Arithmetization/ISigmaOne/G2/Term.lean
@@ -1,0 +1,52 @@
+import Arithmetization.ISigmaOne.PRF
+
+noncomputable section
+
+namespace LO.FirstOrder.Arith.Model
+
+variable {M : Type*} [Zero M] [One M] [Add M] [Mul M] [LT M] [M ⊧ₘ* 𝐈𝚺₁]
+
+namespace FormalizedTerm
+
+variable (M)
+
+/--  -/
+structure FreeStruc where
+  arity : M → M
+
+/--
+
+```lean
+ M:       0 1 2 3 4  5  ...  3 + k   4 + k  5 + k ...
+          : : : : :  :         :       :      :
+ symbols: 0 1 + * #0 #1 ... #(k - 1)   &0     &1  ...
+          : : : : :  :         :       :      :
+ varity:  2 2 4 4 0  0  ...    0       1      1   ...
+```
+ -/
+def Lor : FreeStruc M := ⟨fun x ↦ by {
+
+
+ }⟩
+
+
+
+
+lemma gen_exists (n T : M) :
+  ∃! T' : M, ∀ x : M, x ∈ T' ↔
+    (∃ v < n, x = ⟪0, ⟪0, v⟫⟫) ∨ -- variable
+    (x = ⟪0, ⟪1, 0⟫⟫) ∨          -- constant 0
+    (x = ⟪0, ⟪1, 0⟫⟫) ∨          -- constant 1
+    (∃ t₁ ∈ T, ∃ t₂ ∈ T, x = ⟪2, ⟫)
+     := by {  }
+
+
+def gen (n T : M) : M := T
+
+
+end FormalizedTerm
+
+
+end LO.FirstOrder.Arith.Model
+
+end
